wip

Qsort/Monadic/Terminating.lean
@@ -1,28 +1,32 @@
+import MPL
 import Batteries.Data.List.Perm
 import Batteries.Data.List.Lemmas
 import Qsort.AuxLemmas
 
+open MPL
+
 namespace Monadic
 
-/-- Partitions `as[lo..=hi]`, returning a pivot point and the new array. -/
-@[inline] def qpartition' (as : {as : Array α // as.size = n})
+-- FIXME why do `xs` binders produce errors when importing MPL
+/-- Partitions `xs[lo..=hi]`, returning a pivot point and the new array. -/
+@[inline] def qpartition' (xs : {xs : Array α // xs.size = n})
     (lt : α → α → Bool) (lo hi : Fin n) (hle : lo ≤ hi) :
-    Id $ {as : Array α // as.size = n} × {pivot : Nat // lo ≤ pivot ∧ pivot ≤ hi} := do
+    Idd $ {xs : Array α // xs.size = n} × {pivot : Nat // lo ≤ pivot ∧ pivot ≤ hi} := do
   let mid : Fin n := ⟨(lo.1 + hi) / 2, by omega⟩
   let rec
-  /-- Swaps `lo` and `hi` if needed to ensure `as[lo] ≤ as[hi]`. -/
+  /-- Swaps `lo` and `hi` if needed to ensure `xs[lo] ≤ xs[hi]`. -/
   @[inline] maybeSwap
-      (as : {as : Array α // as.size = n}) (lo hi : Fin n) : {as : Array α // as.size = n} :=
-    let hi := hi.cast as.2.symm
-    let lo := lo.cast as.2.symm
-    if lt (as.1[hi]) (as.1[lo]) then
-      ⟨as.1.swap lo hi, (Array.size_swap ..).trans as.2⟩
-    else as
-  let mut as := as
-  as := maybeSwap as lo mid
-  as := maybeSwap as lo hi
-  as := maybeSwap as hi mid
-  let pivot := as.1[hi.cast as.2.symm]
+      (xs : {xs : Array α // xs.size = n}) (lo hi : Fin n) : {xs : Array α // xs.size = n} :=
+    let hi := hi.cast xs.2.symm
+    let lo := lo.cast xs.2.symm
+    if lt (xs.1[hi]) (xs.1[lo]) then
+      ⟨xs.1.swap lo hi, (Array.size_swap ..).trans xs.2⟩
+    else xs
+  let mut xs := xs
+  xs := maybeSwap xs lo mid
+  xs := maybeSwap xs lo hi
+  xs := maybeSwap xs hi mid
+  let pivot := xs.1[hi.cast xs.2.symm]
   -- we must keep track of i and j and their respective properties all together within a single subtype,
   -- because these dependent properties must be shown in parallel to reassigning the indices
   let mut inv : {t : Nat × Nat // lo ≤ t.1 ∧ t.1 ≤ hi ∧ t.1 ≤ t.2} := ⟨(lo, lo), by omega, by omega⟩
@@ -35,8 +39,8 @@ namespace Monadic
     -- Therefore, showing it is deferred to the correctness proof for now.
     if hjhi : j < hi then
       have _ : i < hi := Nat.lt_of_le_of_lt hij hjhi
-      if lt (as.1[j]) pivot then
-        as := ⟨as.1.swap i j, (Array.size_swap ..).trans as.2⟩
+      if lt (xs.1[j]) pivot then
+        xs := ⟨xs.1.swap i j, (Array.size_swap ..).trans xs.2⟩
         i := i + 1
         j := j + 1
         inv := ⟨(i, j), Nat.le_succ_of_le hloi, by omega, by omega⟩
@@ -44,29 +48,82 @@ namespace Monadic
         j := j + 1
         inv := ⟨(i, j), hloi, by omega, by omega⟩
   let ⟨(i, _), hloi, hihi, _⟩ := inv
-  as := ⟨as.1.swap i hi, (Array.size_swap ..).trans as.2⟩
-  pure ⟨as, ⟨i, hloi, hihi⟩⟩
-  -- loop as lo lo ⟨Nat.le_refl _, Nat.le_refl _, hle⟩
+  xs := ⟨xs.1.swap i hi, (Array.size_swap ..).trans xs.2⟩
+  pure ⟨xs, ⟨i, hloi, hihi⟩⟩
+  -- loop xs lo lo ⟨Nat.le_refl _, Nat.le_refl _, hle⟩
 
 -- hi - lo > hi - mid - 1
 -- - lo > - mid - 1
 -- lo < mid + 1
 -- hi > mid - 1
-def qsort' {n} (lt : α → α → Bool) (as : {as : Array α // as.size = n})
-    (lo : Nat) (hi : Fin n) : Id {as : Array α // as.size = n} := do
+def qsort' {n} (lt : α → α → Bool) (xs : {xs : Array α // xs.size = n})
+    (lo : Nat) (hi : Fin n) : Idd {xs : Array α // xs.size = n} := do
   if h : lo < hi.1 then
-    let ⟨as', mid, (_ : lo ≤ mid), _⟩ :=
-      qpartition' as lt ⟨lo, Nat.lt_trans h hi.2⟩ hi (Nat.le_of_lt h)
-    let mut as := as'
-    as := qsort' lt as lo ⟨mid - 1, by omega⟩
-    as := qsort' lt as (mid + 1) hi
-    pure as
-  else as
+    let ⟨as', mid, (_ : lo ≤ mid), _⟩ ←
+      qpartition' xs lt ⟨lo, Nat.lt_trans h hi.2⟩ hi (Nat.le_of_lt h)
+    let mut xs := as'
+    xs ← qsort' lt xs lo ⟨mid - 1, by omega⟩
+    xs ← qsort' lt xs (mid + 1) hi
+    pure xs
+  else pure xs
 termination_by hi - lo
+#print qsort'._unary
+#print qsort'.eq_def
 
-/-- Sort the array `as[low..=high]` using comparator `lt`. -/
-@[inline] def qsort (as : Array α) (lt : α → α → Bool) :
-    Id (Array α) :=
-  if h : as.size > 0 then
-    (qsort' lt ⟨as, rfl⟩ 0 ⟨as.size - 1, by omega⟩).1
-  else as
+/-- Sort the array `xs[low..=high]` using comparator `lt`. -/
+@[inline] def qsort (xs : Array α) (lt : α → α → Bool) :
+    Idd (Array α) := do
+  if h : xs.size > 0 then
+    pure (← qsort' lt ⟨xs, rfl⟩ 0 ⟨xs.size - 1, by omega⟩).1
+  else pure xs
+
+theorem sorted_triple' (xs : {xs : Array α // xs.size = n})
+    (lo : Nat) (hi : Fin n) (L M R) (hlo : L.length = lo) (hhi : lo + M.length = hi + 1)
+    (hxs : xs.1.toList = L ++ M ++ R)
+    :
+   ⦃⌜True⌝⦄
+   qsort' lt xs lo hi
+   ⦃⇓ xs' => ∃ M', xs'.1.toList = L ++ M' ++ R ∧ M'.Pairwise (fun a b => ¬lt b a)⦄ := by
+  unfold qsort'
+  mintro -
+  mwp
+  split
+  sorry
+  have : lo = hi := sorry
+  have : M.length = 1 := by omega
+  mpure_intro -- TODO should automatically remove `spred`
+  simp only [Bool.not_eq_true, SPred.and_nil, SPred.exists_nil]
+  refine ⟨M, hxs, ?_⟩
+  have : ∃ x, M = [x] := by sorry
+  rw [this.choose_spec]
+  simp
+
+theorem sorted_triple (xs : Array α) :
+   ⦃⌜True⌝⦄
+   qsort xs lt
+   ⦃⇓ xs' => xs'.toList.Pairwise (fun a b => ¬lt b a)⦄
+   := by
+  unfold qsort
+  split
+  . next h =>
+    mintro -
+    mwp
+    -- FIXME why can't I inline the proof as an argument to mspec, with holes for the args corresponding to those of the call to qsort'? Is the pattern matching that it does not powerful enough?
+    have :
+     ⦃⌜True⌝⦄
+     qsort' lt ⟨xs, rfl⟩ 0 ⟨xs.size - 1, by omega⟩
+     ⦃⇓ xs' => ∃ M', xs'.1.toList = [] ++ M' ++ [] ∧ M'.Pairwise (fun a b => ¬lt b a)⦄ :=
+     (sorted_triple' ⟨xs, rfl⟩ 0 ⟨xs.size - 1, by omega⟩ [] xs.toList [] rfl (by simp; omega) (by simp))
+    mspec this
+    mpure h
+    simp_all
+  . next h =>
+    simp at h
+    subst h
+    mintro -
+    mwp
+    simp
+
+theorem sorted (xs : Array α) :
+    (qsort xs lt).run.toList.Pairwise (fun a b => ¬lt b a) := by
+  exact sorted_triple (lt := lt) (α := α) xs True.intro
