Qsort.lean
@@ -1,5 +1,6 @@
 -- This module serves as the root of the `Qsort` library.
 -- Import modules here that should be built as part of the library.
 import Qsort.Pure
-import Qsort.Monadic
+import Qsort.Monadic.Terminating
+import Qsort.Monadic.Partial
 import Qsort.Experiments
